Temporal_Planning_Base/ListMisc.thy
@@ -1,0 +1,117 @@
+theory ListMisc
+  imports "Automatic_Refinement.Misc"
+begin
+
+locale filter_sorted_distinct_list =
+  fixes xs::"nat list"
+    and P::"nat \<Rightarrow> bool"
+    and ys
+  assumes ys: "ys = filter P xs"
+      and sorted: "sorted xs"
+      and distinct: "distinct xs"
+begin
+
+  lemma ys_mono: "ys ! m < ys ! n" if "m < n" "n < length ys" for m n
+    apply (rule distinct_sorted_mono)
+    using that sorted distinct unfolding ys
+    by (auto intro: sorted_filter')
+
+  lemma ys_sorted: "ys ! m \<le> ys ! n" if "m \<le> n" "n < length ys" for m n
+    using that by (cases "m = n") (fastforce dest: le_neq_implies_less ys_mono)+
+
+  lemma ys_mono': "n < m" 
+    if "ys ! n < ys ! m" 
+      "n < length ys" 
+    for m n
+    apply (rule contrapos_pp[OF that(1)])
+    using ys_sorted[OF _ that(2), of m] by simp
+   
+  lemma ys_Suc: "ys ! j < ys ! Suc j" if "Suc j < length ys" for j
+    using ys_mono that by blast
+
+  lemma ys_exI: "\<exists>ij < length ys. ys ! ij = (xs ! j)" 
+    if "j < length xs" 
+       "P (xs ! j)" 
+    for j
+    apply (subst in_set_conv_nth[symmetric])
+    by (simp add: that ys)
+
+
+  lemma length_ys: "length ys \<le> length xs" 
+    unfolding ys 
+    apply (rule order_trans)
+     apply (rule length_filter_le)
+    by simp
+
+  lemma nth_ys_ran: "\<forall>j < length ys. ys ! j \<in> set xs"
+    apply (subst all_set_conv_all_nth[symmetric])
+    unfolding ys by simp
+
+  lemma ys_inc_all: "\<not> P m" 
+    if jl: "Suc j < length ys"
+      and m: "m \<in> set xs"
+      and x: "Suc (ys ! j) \<le> m" "m < ys ! Suc j" 
+    for j m
+  proof (intro notI)
+    assume a: "P m"
+    obtain xm where
+      xm: "xm < length xs"
+      "m = xs ! xm" using in_set_conv_nth m by metis
+    obtain im where
+      im: "im < length ys" "ys ! im = m"
+      using ys_exI xm a by blast
+    hence "ys ! j < ys ! im" "ys ! im < ys ! Suc j" using x by simp_all
+    hence "j < im" "im < Suc j"
+      using jl im(1)
+      by (auto elim!: ys_mono')
+    thus False by simp
+  qed
+
+  lemma ys_inc_all_below: "\<not> (P m)" 
+    if jl: "0 < length ys" 
+      and m: "m \<in> set xs"
+   and x: "m < ys ! 0" for m
+  proof (intro notI)
+    assume a: "P m"
+    obtain xm where
+      xm: "xm < length xs"
+      "m = xs ! xm" using in_set_conv_nth m by metis
+    obtain im where
+      im: "im < length ys" "ys ! im = m"
+      using ys_exI xm a  by blast
+    hence o: "ys ! im < ys ! 0" using x by simp_all
+    have "im < 0"
+      apply (rule ys_mono')
+      using o im by auto
+    thus False by simp
+  qed
+
+  lemma ys_inc_all_above: "\<not> P m" 
+    if x: "ys ! (length ys - 1) < m"
+    and m: "m \<in> set xs" for m
+  proof (cases "length ys = 0")
+    case True
+    then show ?thesis by (auto dest:  arg_cong[where f = set] simp: ys m)
+  next
+    case False
+    show ?thesis 
+    proof (intro notI)
+      from False 
+      have jl: "0 < length ys" by simp
+      assume a: "P m" 
+      obtain xm where
+        xm: "xm < length xs"
+        "m = xs ! xm" using in_set_conv_nth m by metis
+      obtain im where
+        im: "im < length ys" "ys ! im = m"
+        using ys_exI xm a by blast
+      hence o: "ys ! (length ys - 1) < ys ! im" using x by blast
+      have "(length ys - 1) < im"
+        apply (rule ys_mono')
+        using o jl by auto
+      thus False using im by simp
+    qed
+  qed
+end
+
+end
