ROOT
@@ -13,10 +13,9 @@ session TP_Parsing in Parsing =
 
 session Temporal_Planning_Base in Temporal_Planning_Base =
     Containers +
-    sessions
-      KnuthMorrisPratt
     theories
       Base
+      ListMisc
       Temporal_Plans
       Error_List_Monad_Add
 
